# Report of Signals and Systems Lab Assignment 3

Written by HUANG Guanchao, SID 11912309 and GONG Xinrui, SID 11911233.

---

## 4.2

### Basic Problem a

From the given expression of $x(t)$, we can rewrite $x(t)$ into $x(t) = e^{-2t}u(t) + e^{2t}u(-t)$. So $X(j\omega) = \frac{1}{2+j\omega} + \frac{1}{2-j\omega}$, then we standardize the expression into $X(j\omega) = \frac{4}{4+\omega^2}$

### Basic Problem b

---

## 4.5

### Basic Problem a

---

### Basic Problem b

Since we have already know that `b1 = [2 -1]` and `a1 = [1 1.5 0.5]`, we then use `[r1, p1] = residue(a1, b1)` to compute `r1` and `p1`. The result is `r1 = [6 -5]` and `p1 = [-1 -0.5]`.

So we get $H_1(j\omega) = \frac{6}{j\omega+1}+\frac{-5}{j\omega+0.5}$.

The MATLAB script is shown below.

```matlab
b1 = [1 -2];
a1 = [1 3/2 1/2];
[r1, p1] = residue(b1, a1);
```

---

### Basic Problem c

From problem b, where we have already get $H_1(j\omega) = \frac{6}{j\omega+1}+\frac{-5}{j\omega+0.5}$, we can easily get $h_1(t) = (6e^{-t}-5e^{-0.5t})u(t)$. 

And it is easy to see that $H_1(j\omega)$ is integrable.

---

## Intermediate Problem d

We can easily get `a2 = [1 7 16 12]`, `b2 = [3 10 5]`, so `H2 = freqs(b2, a2)`.

The plot is shown below.

![Figure 4.5-d](https://raw.githubusercontent.com/SamuelHuang2019/SigSys-lab/master/figures/A3_4-5_d.png)

The MATLAB script is shown below.

```matlab
b2 = [3 10 5];
a2 = [1 7 16 12];

H2 = freqs(b2, a2);
subplot(2, 1, 1)
semilogy(abs(H2))
title('Magnitude of H2(j\omega)')
xlabel('Frequency ( rad/s )')
ylabel('Magnitude')
subplot(2, 1, 2)
plot(unwrap(angle(H2)))
title('Phase of H2(j\omega)')
xlabel('Frequency ( rad/s )')
ylabel('Phase')
```

---

### Intermediate Problem e

Using the same method as in problem a, `[r2,p2] = residue(b2,a2)`, and `a2 = [1 7 16 12]`, `b2 = [3 10 5]`. We can get `r2 = [2 1 -3]` and `p2 = [-3 -2 -2]`.

So $H_2(j\omega) = \frac{2}{j\omega+3}+\frac{1}{j\omega+2}+\frac{-3}{j\omega+2}$

The MATLAB script is shown below.

```matlab
b2 = [3 10 5];
a2 = [1 7 16 12];
[r2,p2] = residue(b2,a2);
```

---

### Intermediate Problem f

From problem e, where we have already get $H_2(j\omega) = \frac{2}{j\omega+3}+\frac{1}{j\omega+2}+\frac{-3}{j\omega+2}$, we can easily get $h_2(t) = (2e^{-3t}+e^{-2t}-3e^{-2t})u(t)$.

And it is easy to see that $H_2(j\omega)$ is integrable.

---

## Advanced Problem g

